theories/Constants.v
@@ -1,0 +1,97 @@
+From Prototype Require Import Prelude Sig.
+From Prototype Require ParamSyntax.
+
+(** This module exposes various constants to the OCaml plugin.
+    Constants are accessed in the plugin from [plugin/constants.ml]. *)
+
+(** *** Basic constants. *)
+
+Register unit as autosubst.unit.type.
+Register tt as autosubst.unit.tt.
+
+Register prod as autosubst.prod.type.
+Register pair as autosubst.prod.pair.
+
+Register nat as autosubst.nat.type.
+Register O as autosubst.nat.zero.
+Register S as autosubst.nat.succ.
+
+Register list as autosubst.list.type.
+Register nil as autosubst.list.nil.
+Register cons as autosubst.list.cons.
+
+Register string as autosubst.string.type.
+
+Register eq as autosubst.eq.type.
+Register eq_refl as autosubst.eq.eq_refl.
+Register eq_sym as autosubst.eq.eq_sym.
+Register eq_trans as autosubst.eq.eq_trans.
+
+Register eq1 as autosubst.eq1.type.
+Register eq1_refl as autosubst.eq1.refl.
+Register eq1_sym as autosubst.eq1.sym.
+Register eq1_trans as autosubst.eq1.trans.
+
+Register PeanoNat.Nat.measure_induction as autosubst.measure_induction.
+
+(** *** Renamings. *)
+
+Register ren as autosubst.ren.type.
+
+Register rid as autosubst.ren.rid.
+Register rshift as autosubst.ren.rshift.
+Register rcons as autosubst.ren.rcons.
+Register rcomp as autosubst.ren.rcomp.
+Register up_ren as autosubst.ren.up_ren.
+
+Register congr_rcons as autosubst.ren.congr_rcons.
+Register congr_rcomp as autosubst.ren.congr_rcomp.
+Register congr_up_ren as autosubst.ren.congr_up_ren.
+
+(** *** Signatures. *)
+
+Register arg_ty  as autosubst.arg_ty.type.
+Register AT_base as autosubst.arg_ty.base.
+Register AT_term as autosubst.arg_ty.term.
+Register AT_bind as autosubst.arg_ty.bind.
+Register AT_functor as autosubst.arg_ty.functor.
+
+Register kind as autosubst.kind.type.
+Register Kt as autosubst.kind.t.
+Register Ka as autosubst.kind.a.
+Register Kal as autosubst.kind.al.
+
+Register signature as autosubst.signature.type.
+Register Build_signature as autosubst.signature.ctor.
+
+(** *** Parameterized syntax. *)
+
+Register ParamSyntax.expr as autosubst.param.expr.type.
+Register ParamSyntax.E_var as autosubst.param.expr.var.
+Register ParamSyntax.E_ctor as autosubst.param.expr.ctor.
+Register ParamSyntax.E_al_nil as autosubst.param.expr.al_nil.
+Register ParamSyntax.E_al_cons as autosubst.param.expr.al_cons.
+Register ParamSyntax.E_abase as autosubst.param.expr.abase.
+Register ParamSyntax.E_aterm as autosubst.param.expr.aterm.
+Register ParamSyntax.E_abind as autosubst.param.expr.abind.
+Register ParamSyntax.E_afunctor as autosubst.param.expr.afunctor.
+Register ParamSyntax.subst as autosubst.param.subst.
+Register ParamSyntax.esize as autosubst.param.esize.
+
+Register ParamSyntax.rename as autosubst.param.rename.
+Register ParamSyntax.substitute as autosubst.param.substitute.
+Register ParamSyntax.sid as autosubst.param.sid.
+Register ParamSyntax.sshift as autosubst.param.sshift.
+Register ParamSyntax.scons as autosubst.param.scons.
+Register ParamSyntax.up_subst as autosubst.param.up_subst.
+Register ParamSyntax.scomp as autosubst.param.scomp.
+Register ParamSyntax.rscomp as autosubst.param.rscomp.
+Register ParamSyntax.srcomp as autosubst.param.srcomp.
+
+Register ParamSyntax.inv_Kt as autosubst.param.inv_Kt.
+Register ParamSyntax.inv_Kal_nil as autosubst.param.inv_Kal_nil.
+Register ParamSyntax.inv_Kal_cons as autosubst.param.inv_Kal_cons.
+Register ParamSyntax.inv_Ka_term as autosubst.param.inv_Ka_term.
+Register ParamSyntax.inv_Ka_base as autosubst.param.inv_Ka_base.
+Register ParamSyntax.inv_Ka_bind as autosubst.param.inv_Ka_bind.
+Register ParamSyntax.inv_Ka_functor as autosubst.param.inv_Ka_functor.
